

FYS-STK3155/4155, lecture
October 27, 2025

FYS-STK3155/4155 October 27

Solving differential eqs
with Deep learning

$$\frac{dg}{dt} = -\gamma g(t)$$

$$\gamma > 0 \quad t \in [0, \infty)$$

$$g_0 = g(t=0)$$

$$g(t) = g_0 \exp(-\gamma t)$$

$$f(t, g(t), g'(t))$$

$$f(t, g, g') = \frac{dg}{dt} - f(g(t)) = 0$$

in general

$$f(t, g, g', g^{(2)}, \dots, g^{(m)})$$

$$g \Rightarrow g_T(t) = h_1(t) + h_2(t, \underbrace{N(t, \epsilon)})$$

↑
trial

Boundary
+ initial
conditions

neural
network
with
parameters ϵ

$$g(t) = g_0 \exp(-\lambda t)$$

$$g_T(t) = \underbrace{g_0}_{\text{initial condition}} + t N(t, \theta)$$

initial
condition

$$t = 0$$

$$C(\theta) = \frac{1}{n} \sum_{i=0}^{n-1} \left[f(t, g_T, g'_T) \right]^2$$

$g_T(0) = g_0$

$$\hat{\theta} = \underset{\theta}{\operatorname{argmin}} C(\theta)$$

Taylor expansion

$$g(t \pm \Delta t) = g(t) \pm \Delta t \frac{dg}{dt} \Big|_t + \frac{(\Delta t)^2}{2!} \frac{d^2 g}{dt^2} \Big|_t + O(\Delta t^3)$$

Discretize

$$t \rightarrow t_i = t_0 + i \Delta t$$
$$i = 0, 1, 2, \dots, n$$

$$\Delta t = \frac{t_n - t_0}{n}$$

$$g(t + \Delta t) \xrightarrow{n} g(t_i + \Delta t) = g_{i+1}$$

$$g_{i+1} = g_i + \Delta t g'_i + o(\Delta t^2)$$

$$g'_{i+1} \approx g'_i + \Delta t g''_i \Rightarrow$$

$$g'_i \approx \frac{g_{i+1} - g_i}{\Delta t}$$

$$g_1 = g_0 - \delta g_0$$

$$g_2 = g_1 - \delta g_1$$

:

$$g_n = g_{n-1} - \delta g_{n-1}$$

Euler's
method

$$-g''(x) = f(x) \quad \uparrow \text{ known function}$$

$$x \in [0, 1]$$

$$g(x=0) = g(x=1) = 0$$

$$f(x) = (3x + x^2) \exp(x)$$

$$g(x) = x(1-x) \exp(x)$$

$$g_T(x) = x(1-x) N(x, \epsilon)$$

✓

$$g''(x) \approx \frac{g(x+\Delta x) + g(x-\Delta x) - 2g(x)}{(\Delta x)^2}$$

$$g(x) \rightarrow g(x_i) = f_i$$

$$-g''_i = - \left(\frac{g_{i+1} + g_{i-1} - 2g_i}{(\Delta x)^2} \right)$$

$$= f(x_i) = f_i$$

$$g_0 = g_n = 0$$

$$g =$$

$$\begin{bmatrix} g_1 \\ g_2 \\ \vdots \\ g_{n-1} \end{bmatrix}$$

$$A =$$

$$\begin{bmatrix} 2 & -1 & & 0 \\ -1 & 2 & -1 & \\ & -1 & 2 & -1 \\ 0 & & & -1 & 2 \end{bmatrix}$$

$$A \cdot g = \Delta x^2 \cdot f$$

$$g = (A^{-1} \cdot f) \Delta x^2$$

CNNs overarching view



